{
 "cells": [
  {
   "cell_type": "markdown",
   "metadata": {},
   "source": [
    "# Chapter 06 - Exercises"
   ]
  },
  {
   "cell_type": "markdown",
   "metadata": {},
   "source": [
    "### Exercise 6.1\n",
    "\n",
    "**Q**\n",
    "\n",
    "If V changes during the episode, then (6.6) only holds approximately; what would the difference be between the two sides? Let $V_t$ denote the array of state values used at time t in the TD error (6.5) and in the TD update (6.2). Redo the derivation above to determine the additional amount that must be added to the sum of TD errors in order to equal the Monte Carlo error.\n",
    "\n",
    "**A**\n",
    "\n",
    "The equation 6.2, that defines how the values are updated using the TD method, is:\n",
    "\n",
    "\\begin{align*}\n",
    "V(S_t) \\gets V(S_t) + \\alpha [R_{t+1} + \\gamma V(S_{t+1}) - V(S_t)] \\tag{6.2}\n",
    "\\end{align*}\n",
    "\n",
    "The TD error (equation 6.5) is:\n",
    "\n",
    "\\begin{align*}\n",
    "\\delta_t \\stackrel{.}{=} R_{t+1} + \\gamma V(S_{t+1}) - V(S_t) \\tag{6.5}\n",
    "\\end{align*}\n",
    "\n",
    "The equation 6.6 is:\n",
    "\n",
    "\\begin{align*}\n",
    "G_t - V(S_t) &= R_{t+1} + \\gamma G_{t+1} - V(S_t) + \\gamma V(S_{t+1}) - \\gamma V(S_{t+1}) \\tag{from (3.9)} \\\\\n",
    "&= \\delta_t + \\gamma (G_{t+1} - V(S_{t+1})) \\\\\n",
    "&= \\delta_t + \\gamma \\delta_{t+1} + \\gamma^2 (G_{t+2} - V(S_{t+2})) \\\\\n",
    "&= \\delta_t + \\gamma \\delta_{t+1} + \\gamma^2 \\delta_{t+2} + ... + \\gamma^{T-t-1} \\delta_{T-1} + \\gamma^{T-t} (G_T - V(S_T)) \\\\\n",
    "&= \\delta_t + \\gamma \\delta_{t+1} + \\gamma^2 \\delta_{t+2} + ... + \\gamma^{T-t-1} \\delta_{T-1} + \\gamma^{T-t} (0 - 0) \\\\\n",
    "&= \\sum_{k=t}^{T-1} \\gamma^{k-t} \\delta_k \\tag{6.6}\n",
    "\\end{align*}\n",
    "\n",
    "If V changes during the episode, then at the start of time t+1 the new V would be (for TD(0)):\n",
    "\n",
    "\\begin{align*}\n",
    "V_{t+1}(S_t) \\gets V_t(S_t) + \\alpha [R_{t+1} + \\gamma V_t(S_{t+1}) - V_t(S_t)]\n",
    "\\end{align*}\n",
    "\n",
    "where $V_t$ hold the state values at time t.\n",
    "\n",
    "The TD error at time t is now:\n",
    "\n",
    "\\begin{align*}\n",
    "\\delta_t \\stackrel{.}{=} R_{t+1} + \\gamma V_t(S_{t+1}) - V_t(S_t)\n",
    "\\end{align*}\n",
    "\n",
    "The equation 6.6 considering the initial $V_t$ is:\n",
    "\n",
    "\\begin{align*}\n",
    "G_t - V_t(S_t) &= R_{t+1} + \\gamma G_{t+1} - V_t(S_t) + \\gamma V_t(S_{t+1}) - \\gamma V_t(S_{t+1})\\\\\n",
    "&= \\delta_t + \\gamma (G_{t+1} - V_t(S_{t+1})) \\\\\n",
    "&= \\delta_t + \\gamma (G_{t+1} - V_t(S_{t+1}) + V_{t+1}(S_{t+1}) - V_{t+1}(S_{t+1})) \\\\\n",
    "&= \\delta_t + \\gamma (G_{t+1} - V_{t+1}(S_{t+1})) + \\gamma (V_{t+1}(S_{t+1}) - V_t(S_{t+1})) \\\\\n",
    "&= \\delta_t + \\gamma \\delta_{t+1} + \\gamma^2 (G_{t+2} - V_{t+2}(S_{t+2})) + \\gamma^2 (V_{t+2}(S_{t+2}) - V_{t+1}(S_{t+2})) + \\gamma (V_{t+1}(S_{t+1}) - V_t(S_{t+1})) \\\\\n",
    "&= \\delta_t + \\gamma \\delta_{t+1} + \\gamma^2 \\delta_{t+2} + ... + \\gamma^{T-t-1} \\delta_{T-1} + \\gamma^{T-t} (G_T - V_T(S_T)) + \\gamma (V_{t+1}(S_{t+1}) - V_t(S_{t+1})) + \\gamma^2 (V_{t+2}(S_{t+2}) - V_{t+1}(S_{t+2})) + ... + \\gamma^{T-t} (V_T(S_T) - V_{T-1}(S_T)) \\\\\n",
    "&= \\delta_t + \\gamma \\delta_{t+1} + \\gamma^2 \\delta_{t+2} + ... + \\gamma^{T-t-1} \\delta_{T-1} + \\gamma^{T-t} (0 - 0) + \\gamma (V_{t+1}(S_{t+1}) - V_t(S_{t+1})) + \\gamma^2 (V_{t+2}(S_{t+2}) - V_{t+1}(S_{t+2})) + ... + \\gamma^{T-t} (V_T(S_T) - V_{T-1}(S_T)) \\\\\n",
    "&= \\left[ \\sum_{k=t}^{T-1} \\gamma^{k-t} \\delta_k \\right] + \\left[ \\sum_{k=t+1}^{T} \\gamma^{k-t} (V_k(S_k) - V_{k-1}(S_k)) \\right] \\\\\n",
    "&= \\left[ \\sum_{k=t}^{T-1} \\gamma^{k-t} \\delta_k \\right] + \\left[ \\sum_{k=t}^{T-1} \\gamma^{k-t+1} (V_{k+1}(S_{k+1}) - V_k(S_{k+1})) \\right] \\\\\n",
    "&= \\sum_{k=t}^{T-1} [ \\gamma^{k-t} \\delta_k + \\gamma^{k-t+1} (V_{k+1}(S_{k+1}) - V_k(S_{k+1})) ]\n",
    "\\end{align*}\n",
    "\n",
    "We have $V_{k+1}(S_{k+1}) = V_k(S_{k+1})$, unless $S_{k+1} = S_k$, in which case there would be a change in the state-value for the state $S_{k+1} = S_k$ in the transition from the time-step k to k+1, and we would have $V_{k+1}(S_{k+1}) = V_{k+1}(S_k)$, because $S_k = S_{k+1}$. The equation $V_{k+1}(S_{k+1}) = V_k(S_{k+1}) + 1_{S_{k+1} = S_k} (V_{k+1}(S_k) - V_k(S_{k+1}))$ corresponds to these 2 cases. So:\n",
    "\n",
    "\\begin{align*}\n",
    "V_{k+1}(S_{k+1}) &= V_k(S_{k+1}) + 1_{S_{k+1} = S_k} (V_{k+1}(S_k) - V_k(S_{k+1})) \\\\\n",
    "&= V_k(S_{k+1}) + 1_{S_{k+1} = S_k} (V_k(S_k) + \\alpha [R_{k+1} + \\gamma V_k(S_{k+1}) - V_k(S_k)] - V_k(S_{k+1})) \\\\\n",
    "&= V_k(S_{k+1}) + 1_{S_{k+1} = S_k} (V_k(S_k) + \\alpha [R_{k+1} + \\gamma V_k(S_{k+1}) - V_k(S_k)] - V_k(S_k)) \\\\\n",
    "&= V_k(S_{k+1}) + 1_{S_{k+1} = S_k} \\alpha [R_{k+1} + \\gamma V_k(S_{k+1}) - V_k(S_k)] \\\\\n",
    "&= V_k(S_{k+1}) + 1_{S_{k+1} = S_k} \\alpha \\delta_k\n",
    "\\end{align*}\n",
    "\n",
    "We have:\n",
    "\n",
    "\\begin{align*}\n",
    "G_t - V_t(S_t) &= \\sum_{k=t}^{T-1} [ \\gamma^{k-t} \\delta_k + \\gamma^{k-t+1} (V_{k+1}(S_{k+1}) - V_k(S_{k+1})) ] \\\\\n",
    "&= \\sum_{k=t}^{T-1} [ \\gamma^{k-t} \\delta_k + \\gamma^{k-t+1} (V_k(S_{k+1}) + 1_{S_{k+1} = S_k} \\alpha \\delta_k - V_k(S_{k+1})) ] \\\\\n",
    "&= \\sum_{k=t}^{T-1} [ \\gamma^{k-t} \\delta_k + 1_{S_{k+1} = S_k} \\gamma^{k-t+1} \\alpha \\delta_k ]\n",
    "\\end{align*}\n",
    "\n",
    "The above equation is the answer of this question. We can also consider the error using the values after the episode ended (after the terminal state $S_T$ is reached).\n",
    "\n",
    "The final value at the end of the episode, $V_T$, is:\n",
    "\n",
    "\\begin{align*}\n",
    "V(S_t) = V_T(S_t) &= V_{T-1}(S_t) + 1_{S_{T-1} = S_t} \\alpha [R_T + \\gamma V_{T-1}(S_T) - V_{T-1}(S_{T-1})] \\\\\n",
    "&= V_{T-1}(S_t) + 1_{S_{T-1} = S_t} \\alpha \\delta_{T-1} \\\\\n",
    "&= [V_{T-2}(S_t) + 1_{S_{T-2} = S_t} \\alpha \\delta_{T-2}] + 1_{S_{T-1} = S_t} \\alpha \\delta_{T-1} \\\\\n",
    "&= V_t(S_t) + \\alpha \\sum_{k=t}^{T-1} 1_{S_k = S_t} \\delta_k\n",
    "\\end{align*}\n",
    "\n",
    "in which $1_{S_k = S_t}$ means that the value will be 1 if $S_k = S_t$ and 0 otherwise, because $V(S_t)$ changes after the time-step k only if the state at that time-step, $S_k$, is the same state at the time-step t, $S_t$. \n",
    "\n",
    "It's important to keep in mind that the same state may be visited several times depending on the choosen actions and the environment dynamics. For the special case in which we have the state $S_t$ only visited at time t, then $V(S_t) = V_t(S_t) + \\alpha \\delta_t$ (there was only one change: it happened in the transition from t to t+1). In the other extreme, if the state $S_t$ was the only state for all time-steps before the terminal state, then $V(S_t) = V_t(S_t) + \\alpha \\sum_{k=t}^{T-1} \\delta_k$, which is the initial value at time t plus all the changes after each time-step.\n",
    "\n",
    "The new derivation (6.6) is:\n",
    "\n",
    "\\begin{align*}\n",
    "G_t - V(S_t) &= G_t - V_t(S_t) - \\alpha \\sum_{k=t}^{T-1} 1_{S_k = S_t} \\delta_k \\\\\n",
    "&= \\left[ \\sum_{k=t}^{T-1} [ \\gamma^{k-t} \\delta_k + \\gamma^{k-t+1} 1_{S_{k+1} = S_k} \\alpha \\delta_k ] \\right] - \\alpha \\left[ \\sum_{k=t}^{T-1} 1_{S_k = S_t} \\delta_k \\right] \\\\\n",
    "&= \\sum_{k=t}^{T-1} \\left[ \\gamma^{k-t} \\delta_k + \\gamma^{k-t+1} 1_{S_{k+1} = S_k} \\alpha \\delta_k - 1_{S_k = S_t} \\alpha \\delta_k \\right] \\\\\n",
    "&= \\sum_{k=t}^{T-1} \\left[ (\\gamma^{k-t} + \\alpha (1_{S_{k+1} = S_k} \\gamma^{k-t+1} - 1_{S_k = S_t})) \\delta_k \\right]\n",
    "\\end{align*}\n",
    "\n",
    "When $\\alpha$ is infinitesimally small, the above error becomes the Monte Carlo error:\n",
    "\n",
    "\\begin{align*}\n",
    "\\operatorname{lim}_{\\alpha \\to 0} \\sum_{k=t}^{T-1} \\left[ (\\gamma^{k-t} + \\alpha (1_{S_{k+1} = S_k} \\gamma^{k-t+1} - 1_{S_k = S_t})) \\delta_k \\right] = \\sum_{k=t}^{T-1} \\gamma^{k-t} \\delta_k\n",
    "\\end{align*}\n",
    "\n",
    "The above cases were considered for TD(0). For n-step TD, the state-values change only in time-steps multiple of n, so we would have:\n",
    "\n",
    "\\begin{align*}\n",
    "G_t - V(S_t) = \\sum_{k=t}^{T-1} \\left[ (\\gamma^{k-t} + 1_{(k+1) \\equiv 0 \\pmod{n}} \\alpha (1_{S_{k+1} = S_k} \\gamma^{k-t+1} - 1_{S_k = S_t})) \\delta_k \\right]\n",
    "\\end{align*}\n",
    "\n",
    "In the case in which $n \\gt T$, the condition $(k+1) \\equiv 0 \\pmod{n}$ would always be false, and the error above would become the Monte Carlo error, which is expected, because Monte Carlo is equivalent to TD(T+1), as there are T+1 time-steps in t = 0, 1, 2, ..., T-1, T."
   ]
  }
 ],
 "metadata": {
  "language_info": {
   "name": "python"
  }
 },
 "nbformat": 4,
 "nbformat_minor": 2
}
