{
 "cells": [
  {
   "cell_type": "markdown",
   "metadata": {},
   "source": [
    "### Exercise 7.9 \n",
    "\n",
    "**Q**\n",
    "\n",
    "Repeat the above exercise for the action version of the off-policy n-step return (7.14) and the Expected Sarsa TD error (the quantity in brackets in Equation 6.9).\n",
    "\n",
    "**A**\n",
    "\n",
    "Equation 7.14 (to calculate $G_{t:h}$ using the off-policy algorithm with the state-action values) is:\n",
    "\n",
    "\\begin{align*}\n",
    "G_{t:h} &\\doteq R_{t+1} + \\gamma(\\rho_{t+1} G_{t+1:h} + \\overline{V}_{h-1} (S_{t+1}) - \\rho_{t+1} Q_{h-1} (S_{t+1}, A_{t+1})) \\\\\n",
    "&= R_{t+1} + \\gamma \\rho_{t+1} (G_{t+1:h} - Q_{h-1} (S_{t+1}, A_{t+1})) + \\gamma \\overline{V}_{h-1} (S_{t+1}), \\quad t \\lt h \\leq T \\tag{a5}\n",
    "\\end{align*}\n",
    "\n",
    "with $G_{h:h} = Q_{h-1}(S_h, A_h)$ and $G_{T-1:h} \\doteq R_T$.\n",
    "\n",
    "Also, according to 7.8:\n",
    "\n",
    "$$\n",
    "\\overline{V}_t (s) \\doteq \\sum_a \\pi(a | s)Q_t(s, a), \\quad \\forall s \\in \\mathcal{S} \\tag{a4}\n",
    "$$\n",
    "\n",
    "Equation 6.9 is:\n",
    "\n",
    "\\begin{align*}\n",
    "Q(S_t, A_t) &\\gets Q(S_t, A_t) + \\alpha[R_{t+1} + \\gamma \\mathbb{E}_{\\pi}[Q(S_{t+1}, A_{t+1}) | S_{t+1}] - Q(S_t, A_t)] \\\\\n",
    "&\\gets Q(S_t, A_t) + \\alpha \\left[R_{t+1} + \\gamma \\sum_a \\pi(a | S_{t+1}) Q(S_{t+1}, a) - Q(S_t, A_t) \\right]\n",
    "\\end{align*}\n",
    "\n",
    "with the Expected Sarsa TD error being:\n",
    "\n",
    "$$\n",
    "\\delta_t = R_{t+1} + \\gamma \\sum_a \\pi(a | S_{t+1}) Q(S_{t+1}, a) - Q(S_t, A_t) = R_{t+1} + \\gamma \\overline{V} (S_{t+1}) - Q(S_t, A_t)\n",
    "$$\n",
    "\n",
    "Assuming that the approximate state-action value function does not change, that is, $Q_k(S_t, A_t) = Q(S_t, A_t)$ and $\\overline{V}_k (S_t) = \\overline{V} (S_t)$, for all $k$ and for all $t$, and $G_{h:h} = Q(S_h, A_h)$, we have:\n",
    "\n",
    "\\begin{align*}\n",
    "G_{t:h} &= R_{t+1} + \\gamma \\rho_{t+1} (G_{t+1:h} - Q(S_{t+1}, A_{t+1})) + \\gamma \\overline{V} (S_{t+1}) \\\\\n",
    "&= R_{t+1} + \\gamma \\rho_{t+1} (G_{t+1:h} - Q(S_{t+1}, A_{t+1})) + \\gamma \\overline{V} (S_{t+1}) + Q(S_t, A_t) - Q(S_t, A_t) \\\\\n",
    "&= Q(S_t, A_t) + \\delta_t + \\gamma \\rho_{t+1} (G_{t+1:h} - Q(S_{t+1}, A_{t+1})) \\\\\n",
    "G_{t:h} - Q(S_t, A_t) &= \\delta_t + \\gamma \\rho_{t+1} (G_{t+1:h} - Q(S_{t+1}, A_{t+1}))\n",
    "\\end{align*}\n",
    "\n",
    "Making $f(t, h) = G_{t:h} - Q(S_t, A_t)$, with $f(h, h) = G_{h:h} - Q(S_h, A_h) = Q(S_h, A_h) - Q(S_h, A_h) = 0$:\n",
    "\n",
    "\\begin{align*}\n",
    "f(t, h) &= \\delta_t + \\gamma \\rho_{t+1} f(t+1, h) \\\\\n",
    "&= \\delta_t + \\gamma \\rho_{t+1} \\delta_{t+1} + \\gamma^2 \\rho_{t+1} \\rho_{t+2} f(t+2, h) \\\\\n",
    "&= \\delta_t + \\gamma \\rho_{t+1} \\delta_{t+1} + \\gamma^2 \\rho_{t+1} \\rho_{t+2} \\delta_{t+2} + ... + \\gamma^{h-t-1} \\rho_{t+1:h-1} \\delta_{h-1} + \\gamma^{h-t} \\rho_{t+1:h} f(h, h) \\\\\n",
    "&= \\delta_t + \\gamma \\rho_{t+1} \\delta_{t+1} + \\gamma^2 \\rho_{t+1} \\rho_{t+2} \\delta_{t+2} + ... + \\gamma^{h-t-1} \\rho_{t+1:h-1} \\delta_{h-1} + \\gamma^{h-t} \\rho_{t+1:h} \\cdot 0 \\\\\n",
    "&= \\sum_{k=t}^{h-1} \\gamma^{k-t} \\rho_{t+1:k} \\delta_k\n",
    "\\end{align*}\n",
    "\n",
    "So:\n",
    "\n",
    "\\begin{align*}\n",
    "G_{t:h} - Q(S_t, A_t) = \\sum_{k=t}^{h-1} \\gamma^{k-t} \\rho_{t+1:k} \\delta_k\n",
    "\\end{align*}\n",
    "\n",
    "and:\n",
    "\n",
    "\\begin{align*}\n",
    "G_{t:h} = Q(S_t, A_t) + \\sum_{k=t}^{h-1} \\gamma^{k-t} \\rho_{t+1:k} \\delta_k\n",
    "\\end{align*}\n",
    "\n",
    "with $\\rho_{t+1:k} = 1$, if $t \\geq k$.\n"
   ]
  }
 ],
 "metadata": {
  "language_info": {
   "name": "python"
  }
 },
 "nbformat": 4,
 "nbformat_minor": 2
}
